\documentclass[12pt]{article}
\usepackage{amsmath, amssymb, graphicx}
\usepackage{geometry}
\usepackage{enumitem}
\geometry{a4paper, margin=1in}

\begin{document}

\title{Homework 2}
\author{Hao Yin}
\date{\today}
\maketitle

\section*{Question 1}
\begin{enumerate}[label=\roman*.]
    \item (a)
    \[G(s) = \frac{4s-8}{s^2+2s-9}\]
    \[\text{DC GAIN} = G(0) = \frac{-8}{-9}\]

    (b)
    \[G(s) = \frac{10}{s^2+2s+10}\]
    \[\text{DC GAIN} = G(0) = \frac{10}{10} = 1\]

    \item (a)
    \[N(0) = s^2+2s-9 = 0\]
    \[\text{Poles:} s = -1 \pm \sqrt{10}\]
    \[Real(s) = -1 + \sqrt{10} > 0, \text{so this system is unstable.}\]

    (b)
    \[N(0) = s^2+2s+10 = 0\]
    \[\text{Poles:} s = -1 \pm 3i\]
    \[Real(s) = -1 < 0, \text{so this system is stable.}\]

    \item (a)
    
    From TF, we get the ODE:
    \[\ddot{y(t)} + 2\dot{y(t)} - 9y(t) = 4\dot{u(t)} - 8u(t)\]
    Guess that: $y(t) = Ce^{st}, \dot{y(t)} = Cse^{st}, 
        \ddot{y(t)} = Cs^2e^{st}$
    So we get:
    \[Cs^2e^{st} + 2Cse^{st} - 9Ce^{st} = 0\]
    \[Ce^{st} (s^2 + 2s - 9) = 0\]
    \[s = -1 \pm \sqrt{10}\]
    \[y(t) = c_1e^{(-1+\sqrt{10})t} + c_2e^{(-1-\sqrt{10})t}\]

    (b)

    From TF, we get the ODE:
    \[\ddot{y(t)} + 2\dot{y(t)} + 10y(t) = 10u(t)\]
    Guess that: $y(t) = Ce^{st}, \dot{y(t)} = Cse^{st}, 
        \ddot{y(t)} = Cs^2e^{st}$
    So we get:
    \[Cs^2e^{st} + 2Cse^{st} + 10Ce^{st} = 0\]
    \[Ce^{st} (s^2 + 2s + 10) = 0\]
    \[s = -1 \pm 3i\]
    \[y(t) = c_1e^{-t}cos(3t) + c_2e^{-t}sin(3t)\]

    \item (a)
    Roots: $s = -1 \pm \sqrt{10}$

    Homogeneous Solution: 
    \[y_h(t) = c_1e^{(-1+\sqrt{10})t} + c_2e^{(-1-\sqrt{10})t}\]

    Input: $u(t) \equiv 2$

    \[\ddot{y_p(t)} + 2\dot{y_p(t)} - 9y_p(t) = -16\]

    Guess $y_p(t) = C$ , need: $-9C = -16$ ,and then get: $C = \frac{16}{9}$

    So general form of Input response:

    \[y(t) = y_h(t) + y_p(t) = c_1e^{(-1+\sqrt{10})t} + c_2e^{(-1-\sqrt{10})t} + 
        \frac{16}{9}\]

    (b)
    Roots: $s = -1 \pm 3i$

    Homogeneous Solution: 
    \[y(t) = c_1e^{-t}cos(3t) + c_2e^{-t}sin(3t)\]

    Input: $u(t) \equiv 2$

    \[\ddot{y(t)} + 2\dot{y(t)} + 10y(t) = 20\]

    Guess $y_p(t) = C$ , need: $10C = 20$ ,and then get: $C = 2$

    So general form of Input response:

    \[y(t) = y_h(t) + y_p(t) = c_1e^{-t}cos(3t) + c_2e^{-t}sin(3t) + 2\]

    \item (a)
    For the zero initial conditions: $y(0) = 0, \dot{y(0)} = 0$

    We get:
    \[y(0) = c_1 + c_2 + \frac{16}{9} = 0\]
    \[\dot{y(0)} = (-1+\sqrt{10})c_1 + (-1-\sqrt{10}c_2) = 0\]

    So:
    \[c_1 = -1.17, c_2 = -0.6078\]

    So input response:
    \[y(t) = -1.17e^{(-1+\sqrt{10})t} -0.6078e^{(-1-\sqrt{10})t} + 
        \frac{16}{9}\]


    (b)
    For the zero initial conditions: $y(0) = 0, \dot{y(0)} = 0$

    We get:
    \[y(0) = c_1 + 2 = 0\]
    \[\dot{y(0)} = -c_1 + 3c_2 = 0\]

    So:
    \[c_1 = -2, c_2 = -2/3\]

    So input response:
    \[y(t) = -2e^{-t}cos(3t) - \frac{2}{3}e^{-t}sin(3t) + 2\]


\end{enumerate}

\end{document}